Update W15.dfy

Dafny/W15.dfy
@@ -1,3 +1,9 @@
+/**
+In-situ Sorting of Arrays, Classes and Objects
+
+Reg. Program Proofs, Chapter 15-16
+ */
+
 
 /** In-situ sorting */
 
@@ -101,11 +107,11 @@ method SelectionSort(a: array<int>)
 - An object is a stateful abstraction.
   - Includes fields, functions, and methods.
 - Objects are stored on the heap, and passed by reference.
- */
+*/
 
 /**
 Consider a ChecksumMachine object, which computes checksums (essentially hashes) for some data.
-- Provides the functionality to clients to supply data in pieces.
+- Provides the functionality for clients to supply data in pieces.
  */
 
 class ChecksumMachine
@@ -116,7 +122,7 @@ class ChecksumMachine
   // In the compiled code, we will only maintain the running value of the hash     
   var cs: int
 
-  
+  // Helper functions for specification
   ghost function Hash(s: string): int
   {
     SumChars(s) % 137
@@ -129,6 +135,7 @@ class ChecksumMachine
       SumChars(s[..last]) + s[last] as int
   }
 
+  // Invariant connecting the implementation with the specification
   ghost predicate Valid()
     reads this
   {
@@ -136,9 +143,42 @@ class ChecksumMachine
   }
 
   constructor()
-    modifies this
     ensures Valid() && data == ""
   {
     data, cs := "", 0;
   }
+
+  method Append(d: string)
+    requires Valid()
+    modifies this
+    ensures Valid() && data == old(data) + d
+  {
+    var i := 0;
+    while i != |d|
+      invariant 0 <= i <= |d|
+      invariant Valid()
+      invariant data == old(data) + d[0..i]
+    {
+      data := data + d[i..i+1];
+      cs := (cs + (d[i] as int))%137;
+      i := i + 1;
+    }
+  }
+
+  function Checksum() : int
+    requires Valid()
+    reads this
+    ensures Checksum() == Hash(data)
+  {
+    cs
+  }
+}
+
+method Main()
+{
+  var m := new ChecksumMachine();
+  m.Append("green");
+  m.Append("grass");
+  var c := m.Checksum();
+  print "Checksum is ", c, "\n";
 }
